last methods implemented & veriified

Drone.dfy
@@ -17,64 +17,60 @@ class Drone {
 
     var points:seq<(int, int, int)>;
 
-
-
     var curSpeed:int;
     var maxSpeed:int;
-
-
-
-    constructor(r:int, n:int) 
-    requires r > 0 && n > 0
-    ensures RepInv()
-    {
     
-        this.r := r;
-        this.n := n;
-        this.x := 0;
-        this.y := 0;
-        this.z := 0;
-        this.curSpeed := 0;
-        this.maxSpeed := 10;
-        this.points := [];
-        
-
-        
-    }
-
-    function RepInv():bool
+     function RepInv():bool
      reads this`x, this`y, this`z, this`r, this`n, this`curSpeed, this`maxSpeed
     {
         //verify speed
-        0 <= curSpeed <= maxSpeed 
-
-        && 
+        0 <= curSpeed <= maxSpeed && 
         
-        0 <= r && 0 <= n
-
-        &&
-
+        0 < r && 0 < n && 
+        
         verifyBoundaries(x,y,z)
         
         
     }
 
-    function verifyBoundaries(x:int, y:int, z:int) : bool
+    constructor(radius:int, height:int) 
+    requires radius > 0 && height > 0
+    ensures RepInv()
+    {
+    
+        r := radius;
+        n := height;
+        x := 0;
+        y := 0;
+        z := 0;
+        curSpeed := 0;
+        maxSpeed := 10;
+        points := [];
+        
+
+        
+    }
+
+    
+
+    
+
+    function verifyBoundaries(posX:int, posY:int, posZ:int) : bool
     reads this`r, this`n
     {
         //Semisphere
-        ( (x*y)+(y*y)+( (z-n)*(z-n) ) <= (r*r) && n <= z) 
+        ( (posX*posX) + (posY*posY) + ((posZ-n)*(posZ-n) ) <= (r*r) && n <= posZ ) 
         
         || 
         
         //Cylinder
-        ((x*x)+(y*y) <= (r*r) && 0<=z<=n)
+        ( (posX*posX) + (posY*posY) <= (r*r) && 0<=posZ<=n )
     }
 
-    function verifySemisphere(x:int, y:int, z:int) : bool
+    function verifySemisphere(posX:int, posY:int, posZ:int) : bool
     reads this`r, this`n
     {
-        (x*x)+(y*y)+((z-n)*(z-n)) <= (r*r) && n <= z
+        (posX*posX)+(posY*posY)+((posZ-n)*(posZ-n))<=(r*r) && n <= posZ
     }
 
     function verifyIdle() : bool
@@ -108,83 +104,133 @@ class Drone {
     }
     
 
-/*
-    method getX() returns (x:int)
-    {
-        return x;
-    }
 
-    method getY() returns (y:int){
-        return y;
-    }
-
-    method getZ() returns (z:int){
-        return z;
-    }
-*/
-
-    method move(x:int, y:int, z:int)
+    method move(toX:int, toY:int, toZ:int)
     modifies this`targetX, this`targetY, this`targetZ, this`curSpeed
     requires RepInv()
+    requires verifySemisphere(toX, toY, toZ)
     requires verifyIdle()
+    requires z != 0
     ensures RepInv()
+    ensures verifySemisphere(targetX, targetY, targetZ)
     ensures verifyMoving()
+    ensures targetZ != 0
     {
-        targetX := x;
-        targetY := y;
-        targetZ := z;
         curSpeed := maxSpeed;
-
-
+        targetX := toX;
+        targetY := toY;
+        targetZ := toZ;
     }
 
     method completeMove()
+    modifies this`x, this`y, this`z, this`curSpeed
     requires RepInv()
+    requires verifySemisphere(targetX, targetY, targetZ)
+    requires targetZ != 0
+    requires verifyMoving()
+    ensures verifyIdle()
     ensures RepInv()
+    ensures verifySemisphere(x,y,z)
     {
+        curSpeed := 0;
 
+        x := targetX;
+        y := targetY;
+        z := targetZ;
     }
 
-    method addWaypoint()
+    method addWaypoint(toX:int, toY:int, toZ:int)
+    modifies this`points, this`curSpeed
     requires RepInv()
+    requires verifySemisphere(toX, toY, toZ)
+    requires points==[] ==> verifyIdle()
+    requires points!=[] ==> verifyPatrolling()
     ensures RepInv()
     {
-
+        var tuple: (int, int, int) := (toX, toY, toZ);
+        points := points + [tuple];
     }
 
-    method nextWayPoint()
-    requires RepInv()
-    ensures RepInv()
+    method changeWaypoint()
+    modifies this`targetX, this`targetY, this`targetZ, this`points, this`curSpeed
+    requires points!=[]
+    requires verifySemisphere(points[0].0, points[0].1, points[0].2)
+    ensures verifySemisphere(targetX, targetY, targetZ)
     {
+      
+        targetX := points[0].0;
+        targetY :=points[0].1;
+        targetZ :=points[0].2;
+        points := points[1..];
 
+        curSpeed := maxSpeed/2; 
+       
+    }
+
+    method CompleteAddWaypoint()
+    modifies this`x, this`y, this`z, this`curSpeed
+    requires RepInv()
+    requires verifyPatrolling()
+    requires verifySemisphere(targetX, targetY, targetZ)
+    ensures verifySemisphere(x, y, z)
+    ensures points==[] ==> verifyIdle()
+    ensures points!=[] ==> verifyPatrolling()
+    {
+         if(points==[]){
+            curSpeed:=0;
+        }
+        x:=targetX;
+        y:=targetY;
+        z:=targetZ;
+
+       
     }
 
     method takeOff()
+    modifies this`curSpeed
     requires RepInv()
+    requires verifyLanded()
+    ensures verifyMoving()
     ensures RepInv()
     {
-
+        curSpeed := maxSpeed;
     }
 
     method completeTakeOff()
+    modifies this`z, this`curSpeed
     requires RepInv()
+    requires verifyMoving()
+    ensures verifyIdle()
     ensures RepInv()
+    ensures z == n
     {
+        z := n;
 
+        curSpeed := 0;
     }
 
-    method land()
+    method Land()
+    modifies this`curSpeed
     requires RepInv()
+    requires verifyIdle()
+    ensures verifyMoving()
     ensures RepInv()
     {
-
+        curSpeed := maxSpeed;
     }
 
     method completeLand()
+    modifies  this`z, this`curSpeed
     requires RepInv()
+    requires verifyMoving()
+    ensures verifyLanded()
     ensures RepInv()
     {
 
+        z := 0;
+        curSpeed := 0;
     }
+
+    
 
 }
